Auxiliary/Map.dfy
@@ -50,7 +50,15 @@ type Map< T0(==), T1(==) > {
     requires Valid()
     ensures r.Valid()
     ensures r.Model() == Model() - {key}
+    ensures if key !in Keys() then r.Cardinality() == Cardinality()
+            else r.Cardinality() == Cardinality() - 1
+    ensures r.Universe() == Universe()
     ensures counter_out == counter_in + UBSize()
+
+ method {:axiom} PickKey(ghost counter_in:nat) returns (key:T0, ghost counter_out:nat)
+    requires Valid()
+    ensures key in Model().Keys
+    ensures counter_out == counter_in + 1
 
   method {:axiom} nPairs(ghost counter_in:nat) returns (n:int, ghost counter_out:nat)
     requires Valid()
@@ -64,7 +72,7 @@ type Map< T0(==), T1(==) > {
 
   method {:axiom} Empty(ghost counter_in:nat) returns (b:bool, ghost counter_out:nat)
     requires Valid()
-    ensures b == (Model() == map[])//(|Model()| == 0)
+    ensures b == (Model() == map[])
     ensures counter_out == counter_in + 1
 
   method {:axiom} Copy(ghost counter_in:nat) returns (r:Map<T0,T1>, ghost counter_out:nat)
@@ -109,33 +117,42 @@ type Map_Map_T< T0(==), T1(==), T2(==) > {
   { |Model()| }
 
 
-  method {:axiom} Get(key:map<T0, T1>, ghost counter_in:nat) returns (val:T2, ghost counter_out:nat)
+  method {:axiom} Get(key:Map<T0, T1>, ghost counter_in:nat) returns (val:T2, ghost counter_out:nat)
     requires Valid()
-    ensures key in Model().Keys
-    ensures val == Model()[key]
+    ensures key.Model() in Model().Keys
+    ensures val == Model()[key.Model()]
     ensures counter_out == counter_in + UBSize()
 
-  method {:axiom} Insert(key:map<T0, T1>, val:T2, ghost counter_in:nat) returns (r:Map_Map_T<T0,T1,T2>, ghost counter_out:nat)
+  method {:axiom} Insert(key:Map<T0, T1>, val:T2, ghost counter_in:nat) returns (r:Map_Map_T<T0,T1,T2>, ghost counter_out:nat)
     requires Valid()
     ensures r.Valid()
-    ensures r.Model() == Model()[key := val]
-    ensures r.Universe() == Universe()[key := val]
+    ensures r.Model() == Model()[key.Model() := val]
+    ensures r.Universe() == Universe()[key.Model() := val]
     ensures counter_out == counter_in + UBSize()
 
-  method {:axiom} Remove(key:map<T0, T1>, ghost counter_in:nat) returns (r:Map_Map_T<T0,T1,T2>, ghost counter_out:nat)
+  method {:axiom} Remove(key:Map<T0, T1>, ghost counter_in:nat) returns (r:Map_Map_T<T0,T1,T2>, ghost counter_out:nat)
     requires Valid()
     ensures r.Valid()
-    ensures r.Model() == Model() - {key}
+    ensures r.Model() == Model() - {key.Model()}
+    ensures if key.Model() !in Keys() then r.Cardinality() == Cardinality()
+            else r.Cardinality() == Cardinality() - 1
+    ensures r.Universe() == Universe()
     ensures counter_out == counter_in + UBSize()
+
+ method {:axiom} PickKey(ghost counter_in:nat) returns (key:Map<T0, T1>, ghost counter_out:nat)
+    requires Valid()
+    ensures key.Valid()
+    ensures key.Model() in Model().Keys
+    ensures counter_out == counter_in + UBSize_Keys()
 
   method {:axiom} nPairs(ghost counter_in:nat) returns (n:int, ghost counter_out:nat)
     requires Valid()
     ensures n == |Model()|
     ensures counter_out == counter_in + 1
 
-  method {:axiom} ContainsKey(key:map<T0, T1>, ghost counter_in:nat) returns (b:bool, ghost counter_out:nat)
+  method {:axiom} ContainsKey(key:Map<T0, T1>, ghost counter_in:nat) returns (b:bool, ghost counter_out:nat)
     requires Valid()
-    ensures b == (key in Model())
+    ensures b == (key.Model() in Model())
     ensures counter_out == counter_in + UBSize()
 
   method {:axiom} Empty(ghost counter_in:nat) returns (b:bool, ghost counter_out:nat)
@@ -150,4 +167,21 @@ type Map_Map_T< T0(==), T1(==), T2(==) > {
     ensures r.Universe() == Model()
     ensures counter_out == counter_in + UBSize()
 
+}
+
+
+ghost predicate in_universe_Map(M:Map, U:Map)
+{
+  M.Valid() &&
+  U.Valid() &&
+  (M.Universe().Keys <= U.Model().Keys) &&
+  (forall k | k in M.Universe().Keys :: M.Universe()[k] == U.Model()[k])
+}
+
+ghost predicate in_universe_Map_Map_T(M:Map_Map_T, U:Map_Map_T)
+{
+  M.Valid() &&
+  U.Valid() &&
+  (M.Universe().Keys <= U.Model().Keys) &&
+  (forall k | k in M.Universe().Keys :: M.Universe()[k] == U.Model()[k])
 }
