Reduction/PolynomialSetCoverToCDPC.dfy
@@ -6,7 +6,8 @@ include "../Auxiliary/Map.dfy"
 include "../Reduction/ReductionSetCoverToCDPC.dfy"
 
 method SetCoverToCDPC_Method(U:Set<int>, S:SetSet<int>, k:nat) returns (r:(Map_Map_T<int, bool, bool>, Map_Map_T<int, bool, int>, Set<int>, real, real, real, real), ghost counter:nat)
+  requires U.Valid() && S.Valid()
+  ensures r.0.Valid() && r.1.Valid() && r.2.Valid()
   requires forall s | s in S.Model() :: s <= U.Model()
   requires isCover(U.Model(), S.Model())
   ensures (r.0.Model(), r.1.Model(), r.2.Model(), r.3, r.4, r.5, r.6) == SetCoverToCDPC(U.Model(), S.Model(), k)
-
