Verification/VerificationCDPC.dfy
@@ -6,7 +6,8 @@ include "../Auxiliary/Map.dfy"
 include "../Auxiliary/Interview.dfy"
 
 
-method verifyCDPC(f:Map_Map_T<int, bool, bool>, g:Map_Map_T<int, bool, int>, P:Set<int>, a:real, b:real, x:real, y:real, iv:Interview) returns (r:bool, ghost counter:nat)
+method verifyCDPC(f:Map_Map_T<int, bool, bool>, g:Map_Map_T<int, bool, int>, P:Set<int>, a:real, b:real, x:real, y:real, iv:Interview, ghost counter_in:nat) returns (r:bool, ghost counter:nat)
+  decreases iv.Questions()
   requires f.Valid() && g.Valid() && P.Valid() && iv.Valid()
   requires forall c1, c2:candidate |  c1 in f.Keys() && c2 in f.Keys() :: c1.Keys == c2.Keys
   requires f.Keys() == g.Keys()
@@ -15,13 +16,200 @@ method verifyCDPC(f:Map_Map_T<int, bool, bool>, g:Map_Map_T<int, bool, int>, P:S
   requires 0.0 <= x <= y <= 1.0
   ensures r == certificateCDPC(f.Model(), g.Model(), P.Model(), a, b, x, y, iv.Model())
   {
-    counter := 0;
+    counter := counter_in;
     var isEmpty:bool; isEmpty, counter := iv.Empty(counter);
     if (isEmpty) {
-      
+      var nCandidates:int; nCandidates, counter := f.nPairs(counter);
+      if (nCandidates == 0) {
+        return true, counter;
+      }
+      else {
+        var okApt:bool; okApt, counter := correctAptRatio(f, x, y, counter);
+        var okPrivate:bool; okPrivate, counter := correctPrivateRatio(f, P, a, b, counter);
+
+        assert iv.Model() == Null && |f.Model()| != 0;
+        ghost var aptGhost:real :=(|(set isApt:candidate | isApt in f.Keys() && f.Model()[isApt] :: isApt)| as real) / (f.Cardinality() as real);
+        ghost var aptPrivate := forall p:int | p in P.Model() ::
+              (
+                var privateRatio:real := (|(set isPrivate:candidate | isPrivate in f.Keys() && isPrivate[p] :: isPrivate)| as real) / (f.Cardinality() as real);
+                a <= privateRatio <= b
+              );
+        
+        assume okApt == (aptGhost <= x || y <= aptGhost);
+        assume okPrivate == aptPrivate;
+
+        return okApt && okPrivate, counter;
+      }
     }
     else {
+      var question:int; question, counter := iv.Key(counter);
+      var f':Map_Map_T<int, bool, bool>; f', counter := f.Copy(counter);
+      var f'Empty:bool; f'Empty, counter := f'.Empty(counter);
+      var ok:bool := true;
+
+      while (!f'Empty)
+        decreases f'.Cardinality()
+        invariant in_universe_Map_Map_T(f', f)
+        invariant ok == (forall cand:candidate | cand in (f.Keys() - f'.Keys()) :: question in cand.Keys)
+      {
+        f', ok, counter := loopQuestionInCandidates(f, f', question, ok, counter);
+      }
+
+      var f_true:Map_Map_T<int, bool, bool>; f_true, counter := candidatesWithSameAnswer(f, question, true, counter);
+      var f_false:Map_Map_T<int, bool, bool>; f_false, counter := candidatesWithSameAnswer(f, question, false, counter);
+      var g_true:Map_Map_T<int, bool, int>; g_true, counter := candidatesWithSameAnswer(g, question, true, counter);
+      var g_false:Map_Map_T<int, bool, int>; g_false, counter := candidatesWithSameAnswer(g, question, false, counter);
       
+      var iv_true:Interview; iv_true, counter := iv.Get(true, counter);
+      var iv_false:Interview; iv_false, counter := iv.Get(false, counter);
+
+      var b_true:bool; b_true, counter := verifyCDPC(f_true, g_true, P, a, b, x, y, iv_true, counter);
+      var b_false:bool; b_false, counter := verifyCDPC(f_false, g_false, P, a, b, x, y, iv_false, counter);
+      ok := ok && b_true && b_false;
+
+      return ok, counter;
     }
-    assume false;
   }
+
+
+method loopQuestionInCandidates(f:Map_Map_T<int, bool, bool>, f':Map_Map_T<int, bool, bool>, question:int, ok:bool, ghost counter_in:nat) returns (f'':Map_Map_T<int, bool, bool>, ok':bool, ghost counter:nat)
+  requires in_universe_Map_Map_T(f', f)
+  requires ok == (forall cand:candidate | cand in (f.Keys() - f'.Keys()) :: question in cand.Keys)
+  ensures in_universe_Map_Map_T(f'', f)
+  ensures ok' == (forall cand:candidate | cand in (f.Keys() - f''.Keys()) :: question in cand.Keys)
+  ensures f''.Cardinality() == f'.Cardinality() - 1
+{
+  counter := counter_in;
+  var cand:Map<int, bool>; cand, counter := f'.PickKey(counter);
+  f'', counter := f'.Remove(cand, counter);
+  
+  var candHasQuestion:bool; candHasQuestion, counter := cand.ContainsKey(question, counter);
+  ok' := ok && candHasQuestion;
+
+  return f'', ok', counter;
+}
+
+
+method correctAptRatio(f:Map_Map_T<int, bool, bool>, x:real, y:real, ghost counter_in:nat) returns (r:bool, ghost counter:nat)
+  requires f.Valid()
+  requires forall c1, c2:candidate |  c1 in f.Keys() && c2 in f.Keys() :: c1.Keys == c2.Keys
+  requires 0.0 <= x <= y <= 1.0
+  requires f.Cardinality() != 0
+  ensures var aptRatio:real := (|(set isApt:candidate | isApt in f.Keys() && f.Model()[isApt] :: isApt)| as real) / (f.Cardinality() as real);
+          (aptRatio <= x || y <= aptRatio)
+{
+  counter := counter_in;
+  var f':Map_Map_T<int, bool, bool>; f', counter := f.Copy(counter);
+  var f'Empty:bool; f'Empty, counter := f'.Empty(counter);
+  var numApt:int := 0;
+  var numTotal:int := 0;
+
+  while (!f'Empty)
+    decreases f'.Cardinality()
+    invariant in_universe_Map_Map_T(f', f)
+    invariant numTotal == (f.Cardinality() - f'.Cardinality())
+    invariant numApt == |(set isApt:candidate | isApt in (f.Keys() - f'.Keys()) && f.Model()[isApt] :: isApt)|
+  {
+    ghost var f'prev := f';
+    var cand:Map<int, bool>; cand, counter := f'.PickKey(counter);
+    f', counter := f'.Remove(cand, counter);
+    var isApt:bool; isApt, counter := f.Get(cand, counter);
+    if (isApt) {
+      numApt := numApt + 1;
+    }
+    assert numApt == |(set isApt:candidate | isApt in (f.Keys() - f'.Keys()) && f.Model()[isApt] :: isApt)| by {
+      assert f'prev.Keys() == (f'.Keys() + {cand.Model()});
+      assert (f.Keys() - (f'.Keys() + {cand.Model()})) == (f.Keys() - f'.Keys() - {cand.Model()});
+      assert if isApt then numApt == |(set isApt:candidate | isApt in (f.Keys() - f'.Keys() - {cand.Model()}) && f.Model()[isApt] :: isApt)| + 1
+            else           numApt == |(set isApt:candidate | isApt in (f.Keys() - f'.Keys() - {cand.Model()}) && f.Model()[isApt] :: isApt)|;
+      lemma_card_apt_set_when_remove_element(f.Model(), f.Keys() - f'.Keys(), cand.Model());
+    }
+    numTotal := numTotal + 1;
+  }
+
+  var aptRatio:real := (numApt as real) / (numTotal as real);
+  return (aptRatio <= x || y <= aptRatio), counter;   // ???
+}
+
+method correctPrivateRatio(f:Map_Map_T<int, bool, bool>, P:Set<int>, a:real, b:real, ghost counter_in:nat) returns (r:bool, ghost counter:nat)
+  requires f.Valid()
+  requires forall c1, c2:candidate |  c1 in f.Keys() && c2 in f.Keys() :: c1.Keys == c2.Keys
+  requires 0.0 <= a <= b <= 1.0
+  requires forall c:candidate | c in f.Keys() :: (P.Model() <= c.Keys)
+  requires f.Cardinality() != 0
+  ensures forall p:int | p in P.Model() ::
+        (
+          var privateRatio:real := (|(set isPrivate:candidate | isPrivate in f.Keys() && isPrivate[p] :: isPrivate)| as real) / (f.Cardinality() as real);
+          a <= privateRatio <= b
+        )
+/*
+{
+  counter := counter_in;
+
+  var P':Set<int>; P', counter := P.Copy(counter);
+  var p:int; p, counter := P.Pick(counter);
+
+  var f':Map_Map_T<int, bool, bool>; f', counter := f.Copy(counter);
+  var f'Empty:bool; f'Empty, counter := f'.Empty(counter);
+  var numPriv:int := 0;
+  var numTotal:int := 0;
+  
+  while (!f'Empty)
+    decreases f'.Cardinality()
+    invariant in_universe_Map_Map_T(f', f)
+    invariant numTotal == (f.Cardinality() - f'.Cardinality())
+    invariant numPriv == |(set isPrivate:candidate | isPrivate in (f.Keys() - f'.Keys()) && isPrivate[p] :: isPrivate)|
+  {
+    ghost var f'prev := f';
+    var cand:Map<int, bool>; cand, counter := f'.PickKey(counter);
+    f', counter := f'.Remove(cand, counter);
+    var isPrivate:bool; isPrivate, counter := cand.Get(p, counter);
+    if (isPrivate) {
+      numPriv := numPriv + 1;
+    }
+    
+    numTotal := numTotal + 1;
+  }
+
+  var privateRatio:real := (numPriv as real) / (numTotal as real);
+
+  assert forall p:int | p in P.Model() ::
+        (
+          var privateRatio:real := (|(set isPrivate:candidate | isPrivate in f.Keys() && isPrivate[p] :: isPrivate)| as real) / (f.Cardinality() as real);
+          a <= privateRatio <= b
+        );
+
+  return (a <= privateRatio <= b), counter;
+}
+*/
+
+method candidatesWithSameAnswer<T>(f:Map_Map_T<int, bool, T>, question:int, answer:bool, ghost counter_in:nat) returns (f':Map_Map_T<int, bool, T>, ghost counter:nat)
+  requires f.Valid()
+  requires forall c1, c2:candidate |  c1 in f.Keys() && c2 in f.Keys() :: c1.Keys == c2.Keys
+  requires forall c:candidate |  c in f.Keys() :: question in c
+  ensures f'.Model() == (map c:candidate | c in f.Keys() && c[question] == answer :: f.Model()[c])
+
+
+lemma lemma_card_apt_set_when_remove_element(f:map<candidate, bool>, cands:set<candidate>, cand:candidate)
+  requires cand in cands
+  requires cands <= f.Keys
+  ensures if f[cand] then
+            (|(set isApt:candidate | isApt in cands && f[isApt] :: isApt)|
+            ==
+            |(set isApt:candidate | isApt in (cands - {cand}) && f[isApt] :: isApt)| + 1)
+          else
+            |(set isApt:candidate | isApt in cands && f[isApt] :: isApt)|
+            ==
+            |(set isApt:candidate | isApt in (cands - {cand}) && f[isApt] :: isApt)|
+{
+  if f[cand] {
+    assert (set isApt:candidate | isApt in (cands - {cand}) && f[isApt] :: isApt) + {cand}
+            ==
+            (set isApt:candidate | isApt in cands && f[isApt] :: isApt);
+  }
+  else {
+    assert (set isApt:candidate | isApt in (cands - {cand}) && f[isApt] :: isApt)
+            ==
+            (set isApt:candidate | isApt in cands && f[isApt] :: isApt);
+  }
+}
